theories/logrel.v
@@ -112,7 +112,7 @@ Section logrel.
     (match g with
     (* | Local => ⌜related_sts_pub_plus_world W W'⌝ *)
     | Local | Global => ⌜related_sts_priv_world W W'⌝
-    | Monotone => ⌜related_sts_a_world W W' l⌝
+    | Directed => ⌜related_sts_a_world W W' l⌝
      end)%I.
 
   Global Instance future_world_persistent g l W W': Persistent (future_world g l W W').
@@ -145,7 +145,7 @@ Section logrel.
       |          |         nwl           |          pwl           |
       |          | - < a    |    a ≤ -   |  - < a    |    a ≤ -   |
       -------------------------------------------------------------
-      | Monotone | {M,P}    | {M,P,U}    |    {M}    |    {M,U}   |
+      | Directed | {M,P}    | {M,P,U}    |    {M}    |    {M,U}   |
       |-----------------------------------------------------------|
       | Local    |       {P}             |           N/A          |
       |-----------------------------------------------------------|
@@ -164,7 +164,7 @@ Section logrel.
     match l with
      | Local => (std W) !! a = Some Permanent
      | Global => (std W) !! a = Some Permanent
-     | Monotone => (std W) !! a = Some Monotemporary
+     | Directed => (std W) !! a = Some Monotemporary
                   ∨ (std W) !! a = Some Permanent
     end.
 
@@ -208,7 +208,7 @@ Section logrel.
 
   Program Definition interp_cap_RWL (interp : D) : D :=
     λne W w, (match w with
-              | inr ((RWL,Monotone),b,e,a) =>
+              | inr ((RWL,Directed),b,e,a) =>
                 [∗ list] a ∈ (region_addrs b e), (read_write_cond a interp) ∧ ⌜region_state_pwl_mono W a⌝
               (* | inr ((RWL,Local),b,e,a) => *)
               (*   [∗ list] a ∈ (region_addrs b e), ∃ p, ⌜PermFlows RWL p⌝ ∗ (read_write_cond a p interp) ∧ ⌜region_state_pwl W a⌝ *)
@@ -242,7 +242,7 @@ Section logrel.
 
   Program Definition interp_cap_RWLX (interp : D) : D :=
     λne W w, (match w with
-              | inr ((RWLX,Monotone),b,e,a) =>
+              | inr ((RWLX,Directed),b,e,a) =>
                 ([∗ list] a ∈ (region_addrs b e), (read_write_cond a interp)
                                                   ∧ ⌜region_state_pwl_mono W a⌝)
               (* | inr ((RWLX,Local),b,e,a) => *)
@@ -253,9 +253,9 @@ Section logrel.
 
   Program Definition interp_cap_URW (interp : D) : D :=
     λne W w, (match w with
-              | inr ((URW,Monotone),b,e,a) =>
+              | inr ((URW,Directed),b,e,a) =>
                 ([∗ list] a' ∈ (region_addrs b (addr_reg.min a e)), (read_write_cond a' interp)
-                                                                    ∧ ⌜region_state_nwl W a' Monotone⌝) ∗
+                                                                    ∧ ⌜region_state_nwl W a' Directed⌝) ∗
                                              ([∗ list] a' ∈ (region_addrs (addr_reg.max b a) e),                                                                    (read_write_cond a' interp) ∧ ⌜region_state_U_mono W a'⌝)
               | inr ((URW,Local),b,e,a) =>
                 ([∗ list] a' ∈ (region_addrs b (addr_reg.min a e)), (read_write_cond a' interp)
@@ -269,7 +269,7 @@ Section logrel.
 
   Program Definition interp_cap_URWL (interp : D) : D :=
     λne W w, (match w with
-              | inr ((URWL,Monotone),b,e,a) =>
+              | inr ((URWL,Directed),b,e,a) =>
                 ([∗ list] a' ∈ (region_addrs b (addr_reg.min a e)), (read_write_cond a' interp)
                                                                  ∧ ⌜region_state_pwl_mono W a'⌝) ∗
                 ([∗ list] a' ∈ (region_addrs (addr_reg.max b a) e), (read_write_cond a' interp) ∧
@@ -285,9 +285,9 @@ Section logrel.
 
   Program Definition interp_cap_URWX (interp : D) : D :=
     λne W w, (match w with
-              | inr ((URWX,Monotone),b,e,a) =>
+              | inr ((URWX,Directed),b,e,a) =>
                 ([∗ list] a' ∈ (region_addrs b (addr_reg.min a e)), (read_write_cond a' interp)
-                                                                 ∧ ⌜region_state_nwl W a' Monotone⌝)
+                                                                 ∧ ⌜region_state_nwl W a' Directed⌝)
                ∗ ([∗ list] a' ∈ (region_addrs (addr_reg.max b a) e), (read_write_cond a' interp)
                                                                    ∧ ⌜region_state_U_mono W a'⌝)
               | inr ((URWX,Local),b,e,a) =>
@@ -303,7 +303,7 @@ Section logrel.
 
   Program Definition interp_cap_URWLX (interp : D) : D :=
     λne W w, (match w with
-              | inr ((URWLX,Monotone),b,e,a) =>
+              | inr ((URWLX,Directed),b,e,a) =>
                 ([∗ list] a' ∈ (region_addrs b (addr_reg.min a e)), (read_write_cond a' interp)
                                                                  ∧ ⌜region_state_pwl_mono W a'⌝)
                 ∗ ([∗ list] a' ∈ (region_addrs (addr_reg.max b a) e), (read_write_cond a' interp) ∧
@@ -603,15 +603,15 @@ Section logrel.
      [|eauto];solve_addr]).
   Qed.
 
-  Definition isMonotone l :=
+  Definition isDirected l :=
     match l with
-    | Monotone => true
+    | Directed => true
     | _ => false
     end.
 
   Lemma writeLocalAllowed_implies_local W p l b e a:
     pwl p = true ->
-    interp W (inr (p, l, b, e, a)) -∗ ⌜isMonotone l = true⌝.
+    interp W (inr (p, l, b, e, a)) -∗ ⌜isDirected l = true⌝.
   Proof.
     intros. iIntros "Hvalid".
     unfold interp; rewrite fixpoint_interp1_eq /=.
@@ -620,7 +620,7 @@ Section logrel.
 
   Lemma writeLocalAllowedU_implies_local W p l b e a:
     pwlU p = true ->
-    interp W (inr (p, l, b, e, a)) -∗ ⌜isMonotone l = true⌝.
+    interp W (inr (p, l, b, e, a)) -∗ ⌜isDirected l = true⌝.
   Proof.
     intros. iIntros "Hvalid".
     unfold interp; rewrite fixpoint_interp1_eq /=.
@@ -841,7 +841,7 @@ Section logrel.
            ⌜std W !! a = Some Monotemporary⌝.
   Proof.
     intros Hp Hb. iIntros "Hvalid".
-    iAssert (⌜isMonotone l = true⌝)%I as "%". by iApply writeLocalAllowed_implies_local.
+    iAssert (⌜isDirected l = true⌝)%I as "%". by iApply writeLocalAllowed_implies_local.
     eapply withinBounds_le_addr in Hb.
     unfold interp; rewrite fixpoint_interp1_eq /=.
     destruct p; simpl in Hp; try congruence; destruct l;try done.
@@ -856,7 +856,7 @@ Section logrel.
            ⌜std W !! a = Some Monotemporary ∨ ∃ w, std W !! a = Some (Uninitialized w)⌝.
   Proof.
     intros Hp Hb. iIntros "Hvalid".
-    iAssert (⌜isMonotone l = true⌝)%I as "%". by iApply writeLocalAllowedU_implies_local.
+    iAssert (⌜isDirected l = true⌝)%I as "%". by iApply writeLocalAllowedU_implies_local.
     eapply withinBounds_le_addr in Hb.
     unfold interp; rewrite fixpoint_interp1_eq /=.
     destruct p; simpl in Hp; try congruence; destruct l;try done;
@@ -878,7 +878,7 @@ Section logrel.
            ⌜std W !! a' = Some Monotemporary⌝.
   Proof.
     intros Hp Hlt Hb. iIntros "Hvalid".
-    iAssert (⌜isMonotone l = true⌝)%I as "%". by iApply writeLocalAllowedU_implies_local.
+    iAssert (⌜isDirected l = true⌝)%I as "%". by iApply writeLocalAllowedU_implies_local.
     eapply withinBounds_le_addr in Hlt.
     unfold interp; rewrite fixpoint_interp1_eq /=.
     destruct p; simpl in Hp; try congruence; destruct l;try done;
@@ -898,13 +898,13 @@ Section logrel.
                ([∗ list] a ∈ region_addrs b (if isU p && isLocal l then (addr_reg.min a e) else e),
                 (if writeAllowed p || readAllowedU p then read_write_cond a interp else (∃ (P:D), ⌜(∀ Wv, Persistent (P Wv.1 Wv.2))⌝ ∧ read_cond a P interp)) ∧
                       ⌜if pwlU p then region_state_pwl_mono W a else region_state_nwl W a l⌝) ∗
-                (⌜if pwlU p then isMonotone l else True⌝) ∗
+                (⌜if pwlU p then isDirected l else True⌝) ∗
                 (if isU p && isLocal l then [∗ list] a ∈ region_addrs (addr_reg.max b a) e,
                                             read_write_cond a interp ∧
                                                   ⌜if pwlU p
                                                    then region_state_U_pwl_mono W a
                                                    else (match l with
-                                                         | Monotone => region_state_U_mono W a
+                                                         | Directed => region_state_U_mono W a
                                                          | _ => region_state_U W a
                                                          end)⌝ else emp%I))%I).
   Proof.
