theories/binary_model/ftlr_binary/AddSubLt_binary.v
@@ -38,7 +38,7 @@ Section fundamental.
   Lemma add_sub_lt_case (W : WORLD) (r : prodO (leibnizO Reg) (leibnizO Reg)) (p : Perm)
         (g : Locality) (b e a : Addr) (w : Word) (ρ : region_type) (dst : RegName) (r1 r2: Z + RegName) (P:D):
     (∀ w : Word, <[PC:=w]> r.1 = <[PC:=w]> r.2)
-    → p = RX ∨ p = RWX ∨ (p = RWLX /\ g = Monotone)
+    → p = RX ∨ p = RWX ∨ (p = RWLX /\ g = Directed)
     → (∀ x : RegName, is_Some (r.1 !! x) ∧ is_Some (r.2 !! x))
     → isCorrectPC (inr (p, g, b, e, a))
     → (b <= a)%a ∧ (a < e)%a
@@ -60,7 +60,7 @@ Section fundamental.
                        -∗ sts_full_world a0
                           -∗ na_own logrel_nais ⊤
                              -∗ ⤇ Seq (Instr Executable)
-                                -∗ ⌜a2 = RX ∨ a2 = RWX ∨ a2 = RWLX ∧ a3 = Monotone⌝
+                                -∗ ⌜a2 = RX ∨ a2 = RWX ∨ a2 = RWLX ∧ a3 = Directed⌝
                                    → □ region_conditions a0 a2 a3 a4 a5 -∗ interp_conf a0)
     -∗ region_conditions W p g b e
     -∗ (∀ r1 : RegName, ⌜r1 ≠ PC⌝ → fixpoint interp1 W (r.1 !r! r1, r.2 !r! r1))
