theories/binary_model/ftlr_binary/StoreU_binary.v
@@ -207,7 +207,7 @@ Section fundamental.
   Qed.
 
   Lemma execcPC_implies_interp W p g b e a0 :
-    p = RX ∨ p = RWX ∨ p = RWLX ∧ g = Monotone →
+    p = RX ∨ p = RWX ∨ p = RWLX ∧ g = Directed →
     region_conditions W p g b e  -∗
       ((fixpoint interp1) W) (inr (p, g, b, e, a0),inr (p,g,b,e,a0)).
   Proof.
