theories/binary_model/fundamental_binary.v
@@ -76,7 +76,7 @@ Section fundamental.
   Proof. intros. case_decide;apply _. Qed.
 
   Theorem fundamental_binary W r p g b e (a : Addr) :
-    ⊢ ((⌜p = RX⌝ ∨ ⌜p = RWX⌝ ∨ ⌜p = RWLX ∧ g = Monotone⌝) →
+    ⊢ ((⌜p = RX⌝ ∨ ⌜p = RWX⌝ ∨ ⌜p = RWLX ∧ g = Directed⌝) →
        spec_ctx →
        region_conditions W p g b e →
        interp_expression r W (inr ((p,g),b,e,a),inr ((p,g),b,e,a))).
@@ -237,7 +237,7 @@ Section fundamental.
   Qed.
 
   Lemma fundamental_binary_from_interp_correctPC W p g b e a r (w:Word) :
-    p = RX ∨ p = RWX ∨ (p = RWLX ∧ g = Monotone) →
+    p = RX ∨ p = RWX ∨ (p = RWLX ∧ g = Directed) →
     ⊢ spec_ctx -∗ interp W (inr (p, g, b, e, a),w) -∗
       interp_expression r W (inr (p,g,b,e,a),w).
   Proof.
@@ -272,7 +272,7 @@ Section fundamental.
     iDestruct (interp_eq with "Hinterp") as %<-.
     destruct (decide (isCorrectPC (inr ((p,g),b,e,a)))).
     - assert (p = RX ∨ p = RWX ∨ p = RWLX) as Hp;[inversion i;auto|].
-      iAssert (⌜p = RWLX → g = Monotone⌝)%I as %Hmono.
+      iAssert (⌜p = RWLX → g = Directed⌝)%I as %Hmono.
       { iIntros (->). iDestruct (writeLocalAllowed_implies_local with "Hinterp") as %Hmono;[auto|destruct g;auto]. }
       iApply (fundamental_binary_from_interp_correctPC with "Hspec Hinterp").
       destruct Hp as [-> | [-> | ->] ];auto.
