theories/ftlr/interp_weakening.v
@@ -29,14 +29,14 @@ Section fundamental.
                     -∗ region a0
                        -∗ sts_full_world a0
                           -∗ na_own logrel_nais ⊤
-                             -∗ ⌜a2 = RX ∨ a2 = RWX ∨ a2 = RWLX ∧ a3 = Monotone⌝
+                             -∗ ⌜a2 = RX ∨ a2 = RWX ∨ a2 = RWLX ∧ a3 = Directed⌝
                                 → □ region_conditions a0 a2 a3 a4 a5 -∗ interp_conf a0))%I.
 
   (* TODO: Move in monotone ? *)
   Lemma region_state_nwl_future W W' l l' p a a':
     (a < a')%a →
     LocalityFlowsTo l' l ->
-    (if pwlU p then l = Monotone else True) ->
+    (if pwlU p then l = Directed else True) ->
     (@future_world Σ l' a' W W') -∗
     ⌜if pwlU p then region_state_pwl_mono W a else region_state_nwl W a l⌝ -∗
     ⌜region_state_nwl W' a l'⌝.
@@ -71,7 +71,7 @@ Section fundamental.
     (a < a')%a →
     PermFlowsTo p' p ->
     LocalityFlowsTo l' l ->
-    (if pwlU p then l = Monotone else True) ->
+    (if pwlU p then l = Directed else True) ->
     (@future_world Σ l' a' W W') -∗
     ⌜if pwlU p then region_state_pwl_mono W a else region_state_nwl W a l⌝ -∗
     ⌜if pwlU p' then region_state_pwl_mono W' a else region_state_nwl W' a l'⌝.
@@ -233,7 +233,7 @@ Section fundamental.
               case_eq (pwlU p'); intros.
               * assert (pwlU p = true) as HP by (destruct p, p'; naive_solver).
                 rewrite HP in H1. iPureIntro. auto.
-              * iApply (region_state_nwl_future W W Global Monotone _ _ (min a' e')); eauto.
+              * iApply (region_state_nwl_future W W Global Directed _ _ (min a' e')); eauto.
                 assert (x ∈ region_addrs b' (min a' e')) as [_ Hin]%elem_of_region_addrs;
                   [apply elem_of_list_lookup;eauto|];auto.
                 destruct (pwlU p);inversion H0;auto.
@@ -272,7 +272,7 @@ Section fundamental.
               case_eq (pwlU p'); intros.
               * assert (pwlU p = true) as HP by (destruct p, p'; naive_solver).
                 rewrite HP in H1. iPureIntro. auto.
-              * iApply (region_state_nwl_future W W Local Monotone _ _ (min a' e')); eauto.
+              * iApply (region_state_nwl_future W W Local Directed _ _ (min a' e')); eauto.
                 assert (x ∈ region_addrs b' (min a' e')) as [_ Hin]%elem_of_region_addrs;
                   [apply elem_of_list_lookup;eauto|];auto.
                 destruct (pwlU p);inversion H0;auto.
@@ -293,7 +293,7 @@ Section fundamental.
               case_eq (pwlU p'); intros.
               * assert (pwlU p = true) as HP by (destruct p, p'; naive_solver).
                 rewrite HP in H1. iPureIntro. auto.
-              * iApply (region_state_nwl_future W W Monotone Monotone _ _ (min a' e')); eauto.
+              * iApply (region_state_nwl_future W W Directed Directed _ _ (min a' e')); eauto.
                 assert (x ∈ region_addrs b' (min a' e')) as [_ Hin]%elem_of_region_addrs;
                   [apply elem_of_list_lookup;eauto|];auto.
                 destruct (pwlU p);inversion H0;auto.
@@ -351,7 +351,7 @@ Section fundamental.
               case_eq (pwlU p'); intros.
               * assert (pwlU p = true) as HP by (destruct p, p'; naive_solver).
                 rewrite HP in H1. iPureIntro. auto.
-              * iApply (region_state_nwl_future W W l Monotone _ _ (min a' e')); eauto.
+              * iApply (region_state_nwl_future W W l Directed _ _ (min a' e')); eauto.
                 assert (x ∈ region_addrs b' (min a' e')) as [_ Hin]%elem_of_region_addrs;
                   [apply elem_of_list_lookup;eauto|];auto.
                 destruct (pwlU p);auto. destruct l;auto;inversion H0.
